fairness/heap_lang/lm_lsi_hl_wp.v
@@ -22,7 +22,7 @@ Context `{Countable G}.
 (* Context {ifG: fairnessGS iLM Σ}. *)
 Context `{PMPP: @PartialModelPredicatesPre (locale heap_lang) _ _ Σ iM}.
 
-Context {REORDER_PRES: fuel_reorder_preserves_LSI (LSI := LSI)}. 
+(* Context {REORDER_PRES: fuel_reorder_preserves_LSI (LSI := LSI)}.  *)
 
 Let eGS := heap_fairnessGS. 
 
@@ -49,19 +49,21 @@ Local Hint Extern 0 (head_step (CmpXchg _ _ _) _ _ _ _) => eapply CmpXchgS : cor
 Local Hint Extern 0 (head_step (AllocN _ _) _ _ _ _) => apply alloc_fresh : core.
 Local Hint Resolve to_of_val : core.
 
+Notation "'LSGn' Einvs" := (LM_steps_gen_nofork Einvs (EM := EM) (iLM := iLM) (PMPP := PMPP) (eGS := eGS)) (at level 10). 
 Notation "'LSG' Einvs" := (LM_steps_gen Einvs (EM := EM) (iLM := iLM) (PMPP := PMPP) (eGS := eGS)) (at level 10). 
 
 Lemma wp_lift_pure_step_no_fork tid E E' Einvs Φ e1 e2 fs ϕ:
+  LSI_fuel_independent (LSI := LSI) ->
   fs ≠ ∅ ->
   PureExec ϕ 1 e1 e2 ->
   ϕ ->
   (* (PartialModelPredicates Einvs (EM := EM) (iLM := iLM) (PMPP := PMPP) (eGS := eGS)) *)
-  LSG Einvs
+  LSGn Einvs
     ∗
   (|={E}[E']▷=> has_fuels_S tid fs ∗ ((has_fuels tid fs) -∗ WP e2 @ tid; E {{ Φ }}))
   ⊢ WP e1 @ tid; E {{ Φ }}.
-Proof using REORDER_PRES. 
-  intros NnO Hpe Hϕ.
+Proof using. 
+  intros PRES NnO Hpe Hϕ.
   have Hps: pure_step e1 e2.
   { specialize (Hpe Hϕ). by apply nsteps_once_inv in Hpe. }
   iIntros "[#PMP H]". iApply wp_lift_step; eauto.
@@ -106,16 +108,15 @@ Lemma wp_lift_pure_step_no_fork_remove_role
   PureExec ϕ 1 e1 e2 ->
   ϕ ->
   fuel_drop_preserves_LSI s rem (LSI := LSI) ->
-  LSG Einvs ∗
+  LSGn Einvs ∗
   (|={E}[E']▷=> partial_model_is s ∗ has_fuels_S tid fs ∗
                  (partial_model_is s -∗ (has_fuels tid (fs ⇂ (dom fs ∖ rem))) -∗ WP e2 @ tid; E {{ Φ }}))
   ⊢ WP e1 @ tid; E {{ Φ }}.
 Proof using.
-  clear REORDER_PRES. 
   intros NnO Hincl Hdisj Hpe Hϕ PRES. 
   have Hps: pure_step e1 e2.
   { specialize (Hpe Hϕ). by apply nsteps_once_inv in Hpe. }
-  iIntros "[#LSG H]". iApply wp_lift_step; eauto.
+  iIntros "[#LSGn H]". iApply wp_lift_step; eauto.
   { destruct Hps as [Hred _]. specialize (Hred inhabitant). eapply reducible_not_val; eauto. }
   iIntros (extr auxtr K tp1 tp2 σ1 Hvalex Hexend Hloc) "Hsi".
   iMod "H". iMod fupd_mask_subseteq as "Hclose"; last iModIntro; first by set_solver.
@@ -130,7 +131,7 @@ Proof using.
   (* iMod (update_no_step_enough_fuel_drop_gen _ _ _ _ _ rem with "Hfuels Hmod Hmi") as "H"; eauto.  *)
   (*   [by intros X%dom_empty_inv_L | set_solver | econstructor =>//; by apply fill_step |]. *)
 
-  iDestruct (update_no_step_enough_fuel_drop_gen with "LSG") as "HH"; eauto. 
+  iDestruct (update_no_step_enough_fuel_drop_gen with "LSGn") as "HH"; eauto. 
   { by intros X%dom_empty_inv_L. }
   { by rewrite intersection_comm_L. }
   { econstructor =>//; by apply fill_step. }
@@ -156,20 +157,22 @@ Qed.
 (* Proof. *)
 
 Lemma wp_lift_pure_step_no_fork' fs tid E E' Einvs Φ e1 e2:
+  LSI_fuel_independent (LSI := LSI) ->
   fs ≠ ∅ ->
   PureExec True 1 e1 e2 ->
-  LSG Einvs ∗ (|={E}[E']▷=> has_fuels_S tid fs ∗ ((has_fuels tid fs) -∗ WP e2 @ tid; E {{ Φ }}))
+  LSGn Einvs ∗ (|={E}[E']▷=> has_fuels_S tid fs ∗ ((has_fuels tid fs) -∗ WP e2 @ tid; E {{ Φ }}))
   ⊢ WP e1 @ tid; E {{ Φ }}.
-Proof using REORDER_PRES.
+Proof using.
   intros. by iApply wp_lift_pure_step_no_fork.
 Qed.
 
 Lemma wp_lift_pure_step_no_fork_singlerole tid E E' Einvs Φ e1 e2 ρ f φ:
+  LSI_fuel_independent (LSI := LSI) ->
   PureExec φ 1 e1 e2 -> φ ->
-  LSG Einvs ∗ (|={E}[E']▷=> has_fuel tid ρ (S f) ∗ ((has_fuel tid ρ f) -∗ WP e2 @ tid; E {{ Φ }}))
+  LSGn Einvs ∗ (|={E}[E']▷=> has_fuel tid ρ (S f) ∗ ((has_fuel tid ρ f) -∗ WP e2 @ tid; E {{ Φ }}))
   ⊢ WP e1 @ tid; E {{ Φ }}.
-Proof using REORDER_PRES. 
-  iIntros (??) "H". rewrite has_fuel_fuels_S.
+Proof using. 
+  iIntros (???) "H". rewrite has_fuel_fuels_S.
   iApply (wp_lift_pure_step_no_fork {[ ρ := f ]} {[ρ]}); eauto; last first.
   rewrite has_fuel_fuels //. apply map_non_empty_singleton.
 Qed.
@@ -185,12 +188,11 @@ Lemma wp_lift_pure_step_no_fork_take_step_stash s1 s2 tid E E' Einvs fs1 fs2 fr1
   dom fs2 ∩ fr_stash = ∅ ->
   iM.(fmtrans) s1 (Some ρ) s2 ->
   model_step_preserves_LSI s1 ρ s2 fs1 fs2 (LSI := LSI) ->
-  LSG Einvs ∗ (|={E}[E']▷=> partial_model_is s1 ∗ has_fuels tid fs1 ∗ partial_free_roles_are fr1 ∗
+  LSGn Einvs ∗ (|={E}[E']▷=> partial_model_is s1 ∗ has_fuels tid fs1 ∗ partial_free_roles_are fr1 ∗
                  (partial_model_is s2 -∗ partial_free_roles_are (fr1 ∖ (live_roles iM s2 ∖ (live_roles iM s1 ∪ dom fs1 ∩ dom fs2)) ∪ fr_stash)
                   -∗ (has_fuels tid fs2 -∗ WP e2 @ tid; E {{ Φ }})))
   ⊢ WP e1 @ tid; E {{ Φ }}.
 Proof using.
-  clear REORDER_PRES. 
   iIntros (Hpe Hφ Hinvs Hval Hfr ??? Htrans PRES).
   have Hps: pure_step e1 e2.
   { specialize (Hpe Hφ). by apply nsteps_once_inv in Hpe. }
@@ -229,13 +231,12 @@ Lemma wp_lift_pure_step_no_fork_take_step s1 s2 tid E E' Einvs fs1 fs2 fr1 Φ e1
   live_roles iM s2 ∖ live_roles iM s1 ⊆ fr1 ∪ dom fs1 ∩ dom fs2 →
   iM.(fmtrans) s1 (Some ρ) s2 ->
   model_step_preserves_LSI s1 ρ s2 fs1 fs2 (LSI := LSI) ->
-  LSG Einvs ∗
+  LSGn Einvs ∗
   (|={E}[E']▷=> partial_model_is s1 ∗ has_fuels tid fs1 ∗ partial_free_roles_are fr1 ∗
                  (partial_model_is s2 -∗ partial_free_roles_are (fr1 ∖ (live_roles iM s2 ∖ (live_roles iM s1 ∪ dom fs1 ∩ dom fs2)))
                   -∗ (has_fuels tid fs2 -∗ WP e2 @ tid; E {{ Φ }})))
   ⊢ WP e1 @ tid; E {{ Φ }}.
 Proof using.
-  clear REORDER_PRES. 
   iIntros.
   iApply wp_lift_pure_step_no_fork_take_step_stash.
   5: { apply empty_subseteq. }
@@ -253,16 +254,15 @@ Lemma wp_lift_pure_step_no_fork_singlerole_take_step s1 s2 tid E E' Einvs
   live_roles _ s2 ⊆ live_roles _ s1 ->
   (f2 ≤ iLM.(lm_fl) s2)%nat -> iM.(fmtrans) s1 (Some ρ) s2 ->
   model_step_preserves_LSI s1 ρ s2 {[ ρ := f1 ]} fs2 (LSI := LSI) ->
-  LSG Einvs ∗ (|={E}[E']▷=> partial_model_is s1 ∗ partial_free_roles_are fr ∗ has_fuel tid ρ f1 ∗
+  LSGn Einvs ∗ (|={E}[E']▷=> partial_model_is s1 ∗ partial_free_roles_are fr ∗ has_fuel tid ρ f1 ∗
    (partial_model_is s2 -∗ partial_free_roles_are fr -∗ (if decide (ρ ∈ live_roles iM s2) then has_fuel tid ρ f2 else (tid ↦M ∅) ) -∗
                                WP e2 @ tid; E {{ Φ }}))
   ⊢ WP e1 @ tid; E {{ Φ }}.
 Proof using.
-  clear REORDER_PRES. 
   iIntros (Hpe Hφ Hinvs Hroles Hfl Hmdl PRES).
   rewrite has_fuel_fuels.
-  iIntros "[LSG H]".
-  iApply (wp_lift_pure_step_no_fork_take_step _ _ _ _ _ _ {[ρ := f1]} fs2 fr  with "[LSG H]"); eauto.
+  iIntros "[LSGn H]".
+  iApply (wp_lift_pure_step_no_fork_take_step _ _ _ _ _ _ {[ρ := f1]} fs2 fr  with "[LSGn H]"); eauto.
   - subst fs2. repeat split.
     + intros ?. rewrite decide_True //. rewrite lookup_singleton //=. 
     + destruct (decide (ρ ∈ live_roles _ s2)); set_solver.
@@ -282,12 +282,13 @@ Proof using.
 Qed.
 
 Lemma wp_lift_pure_step_no_fork_singlerole' tid E E' Einvs Φ e1 e2 ρ f:
+  LSI_fuel_independent (LSI := LSI) ->
   PureExec True 1 e1 e2 ->
-  LSG Einvs ∗ (|={E}[E']▷=> has_fuel tid ρ (S f) ∗ ((has_fuel tid ρ f) -∗ WP e2 @ tid; E {{ Φ }}))
+  LSGn Einvs ∗ (|={E}[E']▷=> has_fuel tid ρ (S f) ∗ ((has_fuel tid ρ f) -∗ WP e2 @ tid; E {{ Φ }}))
   ⊢ WP e1 @ tid; E {{ Φ }}.
-Proof using REORDER_PRES.
-  iIntros (?) "H". rewrite has_fuel_fuels_S.
-  iApply (wp_lift_pure_step_no_fork' {[ ρ := f ]} {[ρ]}); last first.
+Proof using.
+  iIntros (??) "H". rewrite has_fuel_fuels_S.
+  iApply (wp_lift_pure_step_no_fork' {[ ρ := f ]} {[ρ]}); auto; last first.
   rewrite has_fuel_fuels //. apply map_non_empty_singleton.
 Qed.
 
@@ -300,14 +301,15 @@ Qed.
 (** Fork: Not using Texan triples to avoid some unnecessary [True] *)
 Lemma wp_fork_nostep s tid E Einvs e Φ R1 R2
   (fs: gmap (fmrole iM) nat) (Hdisj: R1 ## R2) (Hnemp: fs ≠ ∅):
+  fuel_reorder_preserves_LSI (LSI := LSI) ->
   R1 ∪ R2 = dom fs ->
   LSG Einvs ∗ (∀ tid', ▷ (has_fuels tid' (fs ⇂ R2) -∗
                 WP e @ s; tid'; ⊤ {{ _, partial_mapping_is {[ tid' := ∅ ]}  }})
   ) -∗
      ▷ (has_fuels tid (fs ⇂ R1) ={E}=∗ Φ (LitV LitUnit)) -∗
      has_fuels_S tid fs -∗ WP Fork e @ s; tid; E {{ Φ }}.
-Proof using REORDER_PRES.
-  iIntros (Hunioneq) "[PMP He] HΦ Htid". iApply wp_lift_atomic_head_step; [done|].
+Proof using.
+  iIntros (? Hunioneq) "[PMP He] HΦ Htid". iApply wp_lift_atomic_head_step; [done|].
   iIntros (extr auxtr K tp1 tp2 σ1 Hvalex Hexend Hloc) "(% & Hsi & Hmi)".
   iMod (update_fork_split_gen R1 R2 _
        (tp1 ++ ectx_language.fill K (Val $ LitV LitUnit) :: tp2 ++ [e]) fs _ _ _ e _ σ1 with "PMP Htid Hmi")
@@ -340,16 +342,17 @@ Lemma wp_fork_nostep_alt s tid E Einvs e Φ
   (fs1 fs2: gmap (fmrole iM) nat)
   (DISJ: fs1 ##ₘ fs2)
   (NE: fs1 ∪ fs2 ≠ ∅):
+  fuel_reorder_preserves_LSI (LSI := LSI) ->
   LSG Einvs ∗ (∀ tid', ▷ (has_fuels tid' fs2 -∗
                 WP e @ s; tid'; ⊤ {{ _, partial_mapping_is {[ tid' := ∅ ]}  }})
   ) -∗
      ▷ (has_fuels tid fs1 ={E}=∗ Φ (LitV LitUnit)) -∗
      has_fuels_S tid (fs1 ∪ fs2) -∗ WP Fork e @ s; tid; E {{ Φ }}.
-Proof using REORDER_PRES.
-  iIntros "[PMP FORK] FUEL1 FUEL".
+Proof using.
+  iIntros (?) "[PMP FORK] FUEL1 FUEL".
   iApply (wp_fork_nostep with "[PMP FORK] [FUEL1]").
   { by eapply map_disjoint_dom_1. }
-  1, 2: set_solver.
+  1, 2, 3: set_solver.
   3: done. 
   { iFrame. iIntros (?). iNext. iIntros "FUEL". iApply "FORK".
     iApply has_fuels_proper; [reflexivity| | iFrame].
@@ -358,18 +361,19 @@ Proof using REORDER_PRES.
   iNext. iIntros "FUEL". iApply "FUEL1".
   iApply has_fuels_proper; [reflexivity| | iFrame].
   by apply leibniz_equiv_iff, gmap_filter_disj_id.
-Qed.   
+Qed.
 
 
 Lemma wp_allocN_seq_nostep s tid E Einvs v n fs:
+  LSI_fuel_independent (LSI := LSI) ->
   fs ≠ ∅ ->
   0 < n →
-  LSG Einvs ⊢
+  LSGn Einvs ⊢
   {{{ has_fuels_S tid fs }}} AllocN (Val $ LitV $ LitInt $ n) (Val v) @ s; tid; E
   {{{ l, RET LitV (LitLoc l); has_fuels tid fs ∗ [∗ list] i ∈ seq 0 (Z.to_nat n),
       (l +ₗ (i : nat)) ↦ v ∗ meta_token (l +ₗ (i : nat)) ⊤ }}}.
-Proof using REORDER_PRES.
-  iIntros (HnO Hn) "#PMP".
+Proof using.
+  iIntros (? HnO Hn) "#PMP".
   iIntros (Φ). iModIntro. iIntros "HfuelS HΦ".
   iApply wp_lift_atomic_head_step_no_fork; auto.
   iIntros (extr auxtr K tp1 tp2 σ1 Hvalex Hexend Hloc) "(% & Hsi & Hmi)".
@@ -396,21 +400,23 @@ Proof using REORDER_PRES.
 Qed.
 
 Lemma wp_alloc_nostep s tid E Einvs v fs :
+  LSI_fuel_independent (LSI := LSI) ->
   fs ≠ ∅ ->
-  LSG Einvs ⊢ {{{ has_fuels_S tid fs }}} Alloc (Val v) @ s; tid; E {{{ l, RET LitV (LitLoc l); l ↦ v ∗ meta_token l ⊤ ∗ has_fuels tid fs }}}.
-Proof using REORDER_PRES. 
-  iIntros (?) "#PMP". iModIntro. iIntros (Φ) "HfuelS HΦ".
+  LSGn Einvs ⊢ {{{ has_fuels_S tid fs }}} Alloc (Val v) @ s; tid; E {{{ l, RET LitV (LitLoc l); l ↦ v ∗ meta_token l ⊤ ∗ has_fuels tid fs }}}.
+Proof using. 
+  iIntros (??) "#PMP". iModIntro. iIntros (Φ) "HfuelS HΦ".
   iApply (wp_allocN_seq_nostep with "PMP HfuelS"); auto with lia.
   iIntros "!>" (l) "/= (? & ? & _)". rewrite loc_add_0. by iApply "HΦ"; iFrame.
 Qed.
 
 Lemma wp_choose_nat_nostep s tid E Einvs fs :
+  LSI_fuel_independent (LSI := LSI) ->
   fs ≠ ∅ ->
-  LSG Einvs ⊢ {{{ has_fuels_S tid fs }}}
+  LSGn Einvs ⊢ {{{ has_fuels_S tid fs }}}
     ChooseNat @ s; tid; E
   {{{ (n:nat), RET LitV (LitInt n); has_fuels tid fs }}}.
-Proof using REORDER_PRES. 
-  iIntros (?). iIntros "#PMP". iModIntro. iIntros (Φ) "HfuelS HΦ". iApply wp_lift_atomic_head_step_no_fork; auto.
+Proof using. 
+  iIntros (??). iIntros "#PMP". iModIntro. iIntros (Φ) "HfuelS HΦ". iApply wp_lift_atomic_head_step_no_fork; auto.
   iIntros (extr auxtr K tp1 tp2 σ1 Hvalex Hexend Hloc) "(% & Hsi & Hmi)".
   iModIntro; iSplit; eauto.
   (* TODO: Improve this so we hide the (arbitrary) choice of `n` *)
@@ -429,10 +435,11 @@ Proof using REORDER_PRES.
 Qed.
 
 Lemma wp_load_nostep s tid E Einvs l q v fs:
+  LSI_fuel_independent (LSI := LSI) ->
   fs ≠ ∅ ->
-  LSG Einvs ⊢ {{{ ▷ l ↦{q} v ∗ has_fuels_S tid fs }}} Load (Val $ LitV $ LitLoc l) @ s; tid; E {{{ RET v; l ↦{q} v ∗ has_fuels tid fs }}}.
-Proof using REORDER_PRES. 
-  iIntros (?). iIntros "#PMP". iModIntro. iIntros (Φ) "[>Hl HfuelS] HΦ". iApply wp_lift_atomic_head_step_no_fork; auto.
+  LSGn Einvs ⊢ {{{ ▷ l ↦{q} v ∗ has_fuels_S tid fs }}} Load (Val $ LitV $ LitLoc l) @ s; tid; E {{{ RET v; l ↦{q} v ∗ has_fuels tid fs }}}.
+Proof using. 
+  iIntros (??). iIntros "#PMP". iModIntro. iIntros (Φ) "[>Hl HfuelS] HΦ". iApply wp_lift_atomic_head_step_no_fork; auto.
   iIntros (extr atr K tp1 tp2 σ1 Hval Hexend Hloc) "(% & Hsi & Hmi) !>".
   iDestruct (@gen_heap_valid with "Hsi Hl") as %Hheap.
   iSplit; first by rewrite Hexend // in Hheap;  eauto. iIntros "!>" (e2 σ2 efs Hstep).
@@ -448,12 +455,13 @@ Proof using REORDER_PRES.
 Qed.
 
 Lemma wp_store_nostep s tid E Einvs l v' v fs:
+  LSI_fuel_independent (LSI := LSI) ->
   fs ≠ ∅ ->
-  LSG Einvs ⊢ {{{ ▷ l ↦ v' ∗ has_fuels_S tid fs }}}
+  LSGn Einvs ⊢ {{{ ▷ l ↦ v' ∗ has_fuels_S tid fs }}}
     Store (Val $ LitV (LitLoc l)) (Val v) @ s; tid; E
   {{{ RET LitV LitUnit; l ↦ v ∗ has_fuels tid fs }}}.
-Proof using REORDER_PRES. 
-  iIntros (?). iIntros "#PMP". iModIntro. iIntros (Φ) "[>Hl HfuelS] HΦ".
+Proof using. 
+  iIntros (??). iIntros "#PMP". iModIntro. iIntros (Φ) "[>Hl HfuelS] HΦ".
   iApply wp_lift_atomic_head_step_no_fork; auto.
   iIntros (extr atr K tp1 tp2 σ1 Hval Hexend Hloc) "(% & Hsi & Hmi) !>".
   iDestruct (@gen_heap_valid with "Hsi Hl") as %Hheap.
@@ -481,7 +489,7 @@ Lemma wp_store_step_keep s tid ρ (fs1 fs2: gmap (fmrole iM) nat) fr fr_stash s1
   (NSL : live_roles iM s1 ∩ (fr_stash ∖ {[ρ]}) = ∅)
   (NOS2 : dom fs2 ∩ fr_stash = ∅)
   (PRES: model_step_preserves_LSI s1 ρ s2 fs1 fs2 (LSI := LSI)):
-  LSG Einvs ⊢
+  LSGn Einvs ⊢
   {{{ ▷ l ↦ v' ∗ ▷ partial_model_is s1 ∗ ▷ has_fuels tid fs1 ∗
       ▷ partial_free_roles_are fr}}}
     Store (Val $ LitV $ LitLoc l) (Val v) @ s; tid; E
@@ -520,7 +528,7 @@ Lemma wp_store_step_singlerole_keep s tid ρ (f1 f2: nat) (* fr *) s1 s2 E Einvs
   (ρ ∉ live_roles iM s2 -> (f2 < f1)%nat ) -> (* TODO: check Zombie case in must_decrease *)
   live_roles _ s2 ⊆ live_roles _ s1 ->
   model_step_preserves_LSI s1 ρ s2 {[ ρ := f1 ]} {[ ρ := f2 ]} (LSI := LSI) ->
-  LSG Einvs ⊢ {{{ ▷ l ↦ v' ∗ ▷ partial_model_is s1 ∗ ▷ has_fuel tid ρ f1
+  LSGn Einvs ⊢ {{{ ▷ l ↦ v' ∗ ▷ partial_model_is s1 ∗ ▷ has_fuel tid ρ f1
         (* ∗ ▷ partial_free_roles_are fr *)
   }}}
     Store (Val $ LitV $ LitLoc l) (Val v) @ s; tid; E
@@ -528,7 +536,6 @@ Lemma wp_store_step_singlerole_keep s tid ρ (f1 f2: nat) (* fr *) s1 s2 E Einvs
                           (* partial_free_roles_are fr ∗ *)
       has_fuel tid ρ f2 }}}. 
 Proof using.
-  clear REORDER_PRES.
   iIntros (Hinvs Hfl Htrans Hdecr ? PRES).
   iIntros "#PMP". iModIntro. iIntros (Φ) "(>Hl & >Hst & >Hfuel1) HΦ".
   iApply wp_lift_atomic_head_step_no_fork; auto.
@@ -573,12 +580,11 @@ Lemma wp_store_step_singlerole s tid ρ (f1 f2: nat) s1 s2 E Einvs l v' v
   f2 ≤ iLM.(lm_fl) s2 -> fmtrans iM s1 (Some ρ) s2 ->
   live_roles _ s2 ⊆ live_roles _ s1 ->
   model_step_preserves_LSI s1 ρ s2 {[ ρ := f1 ]} fs2 (LSI := LSI) ->
-  LSG Einvs ⊢ {{{ ▷ l ↦ v' ∗ ▷ partial_model_is s1 ∗ ▷ has_fuel tid ρ f1}}}
+  LSGn Einvs ⊢ {{{ ▷ l ↦ v' ∗ ▷ partial_model_is s1 ∗ ▷ has_fuel tid ρ f1}}}
     Store (Val $ LitV $ LitLoc l) (Val v) @ s; tid; E
   {{{ RET LitV LitUnit; l ↦ v ∗ partial_model_is s2 ∗ 
       (if decide (ρ ∈ live_roles iM s2) then has_fuel tid ρ f2 else tid ↦M ∅ ∗ partial_free_roles_are {[ ρ ]}) }}}.
 Proof using.
-  clear REORDER_PRES. 
   iIntros (Hinvs Hfl Htrans ? PRES). iIntros "#PMP". iModIntro. iIntros (Φ) "(>Hl & >Hst & >Hfuel1) HΦ".
   iApply wp_lift_atomic_head_step_no_fork; auto.
   iIntros (extr atr K tp1 tp2 σ1 Hval Hexend Hloc) "(% & Hsi & Hmi) !>".
@@ -628,11 +634,10 @@ Lemma wp_cmpxchg_fail_step_singlerole s tid ρ (f1 f2: nat) fr s1 s2 E Einvs l q
   v' ≠ v1 → vals_compare_safe v' v1 → f2 ≤ iLM.(lm_fl) s2 -> iM.(fmtrans) s1 (Some ρ) s2 ->
   live_roles _ s2 ⊆ live_roles _ s1 ->
   model_step_preserves_LSI s1 ρ s2 {[ ρ := f1 ]} fs2 (LSI := LSI) ->
-  LSG Einvs ⊢ {{{ ▷ l ↦{q} v' ∗ ▷ partial_model_is s1 ∗ ▷ has_fuel tid ρ f1 ∗ ▷ partial_free_roles_are fr }}} CmpXchg (Val $ LitV $ LitLoc l) (Val v1) (Val v2) @ s; tid; E
+  LSGn Einvs ⊢ {{{ ▷ l ↦{q} v' ∗ ▷ partial_model_is s1 ∗ ▷ has_fuel tid ρ f1 ∗ ▷ partial_free_roles_are fr }}} CmpXchg (Val $ LitV $ LitLoc l) (Val v1) (Val v2) @ s; tid; E
   {{{ RET PairV v' (LitV $ LitBool false); l ↦{q} v' ∗ partial_model_is s2 ∗ partial_free_roles_are fr ∗
       (if decide (ρ ∈ live_roles iM s2) then has_fuel tid ρ f2 else tid ↦M ∅ ) }}}.
 Proof using.
-  clear REORDER_PRES.
   iIntros (Hinvs ?? Hfl Htrans ? PRES) "#PMP". iModIntro. iIntros (Φ) "(>Hl & >Hst & >Hfuel1 & > Hfr) HΦ". iApply wp_lift_atomic_head_step_no_fork; auto.
   iIntros (extr atr K tp1 tp2 σ1 Hval Hexend Hloc) "(% & Hsi & Hmi) !>".
   iDestruct (@gen_heap_valid with "Hsi Hl") as %Hheap.
@@ -674,12 +679,11 @@ Lemma wp_cmpxchg_suc_step_singlerole_keep_dead  s tid ρ (f1 f2: nat) fr s1 s2 E
   v' = v1 → vals_compare_safe v' v1 → f2 < f1 -> iM.(fmtrans) s1 (Some ρ) s2 ->
   live_roles _ s2 ⊆ live_roles _ s1 ->
   model_step_preserves_LSI s1 ρ s2 {[ ρ := f1 ]} {[ ρ := f2 ]} (LSI := LSI) ->
-  LSG Einvs ⊢ {{{ ▷ l ↦ v' ∗ ▷ partial_model_is s1 ∗ ▷ has_fuel tid ρ f1 ∗ ▷ partial_free_roles_are fr }}}
+  LSGn Einvs ⊢ {{{ ▷ l ↦ v' ∗ ▷ partial_model_is s1 ∗ ▷ has_fuel tid ρ f1 ∗ ▷ partial_free_roles_are fr }}}
     CmpXchg (Val $ LitV $ LitLoc l) (Val v1) (Val v2) @ s; tid; E
   {{{ RET PairV v' (LitV $ LitBool true); l ↦ v2 ∗ partial_model_is s2 ∗ partial_free_roles_are fr ∗
       has_fuel tid ρ f2 }}}.
 Proof using.
-  clear REORDER_PRES.
   iIntros (Hinvs ??? Hfl Htrans ? PRES) "#PMP". iModIntro. iIntros (Φ) "(>Hl & >Hst & >Hfuel1 & >Hfr) HΦ".
   iApply wp_lift_atomic_head_step_no_fork; auto.
   iIntros (extr atr K tp1 tp2 σ1 Hval Hexend Hloc) "(% & Hsi & Hmi) !>".
@@ -715,12 +719,11 @@ Lemma wp_cmpxchg_suc_step_singlerole s tid ρ (f1 f2: nat) fr s1 s2 E Einvs l v'
   v' = v1 → vals_compare_safe v' v1 → f2 ≤ iLM.(lm_fl) s2 -> iM.(fmtrans) s1 (Some ρ) s2 ->
   live_roles _ s2 ⊆ live_roles _ s1 ->
   model_step_preserves_LSI s1 ρ s2 {[ ρ := f1 ]} fs2 (LSI := LSI) ->
-  LSG Einvs ⊢ {{{ ▷ l ↦ v' ∗ ▷ partial_model_is s1 ∗ ▷ has_fuel tid ρ f1 ∗ ▷ partial_free_roles_are fr }}}
+  LSGn Einvs ⊢ {{{ ▷ l ↦ v' ∗ ▷ partial_model_is s1 ∗ ▷ has_fuel tid ρ f1 ∗ ▷ partial_free_roles_are fr }}}
     CmpXchg (Val $ LitV $ LitLoc l) (Val v1) (Val v2) @ s; tid; E
   {{{ RET PairV v' (LitV $ LitBool true); l ↦ v2 ∗ partial_model_is s2 ∗ partial_free_roles_are fr ∗
       (if decide (ρ ∈ live_roles iM s2) then has_fuel tid ρ f2 else tid ↦M ∅ ) }}}.
 Proof using.
-  clear REORDER_PRES. 
   iIntros (Hinvs ?? Hfl Htrans ? PRES) "#PMP". iModIntro. iIntros (Φ) "(>Hl & >Hst & >Hfuel1 & >Hfr) HΦ".
   iApply wp_lift_atomic_head_step_no_fork; auto.
   iIntros (extr atr K tp1 tp2 σ1 Hval Hexend Hloc) "(% & Hsi & Hmi) !>".
